wip

testsuite/tests/coqgen/cocti_defs.v
@@ -205,13 +205,13 @@ Definition bounded_nat_of_int (m : nat) (n : int) : M nat :=
 
 Fixpoint forloop (h : nat) (n_1 n_2 : int) (b : int -> M unit) : M unit :=
   if h is h.+1 then
-    if Sint63.compare n_1 n_2 is Gt then Ret tt
+    if ltsb n_2 n_1 then Ret tt
     else (do _ <- b n_1; forloop h (n_1 + 1)%sint63 n_2 b)
   else FailGas.
 
 Fixpoint downforloop (h : nat) (n_1 n_2 : int ) (b : int -> M unit) : M unit :=
   if h is h.+1 then
-    if Sint63.compare n_1 n_2 is Lt then Ret tt
+    if ltsb n_1 n_2 then Ret tt
     else (do _ <- b n_1; downforloop h (n_1 - 1)%sint63 n_2 b)
   else FailGas.
 
